More work on Stuck.v

Stuck.v
@@ -1,114 +1,26 @@
 Require Import Fiat.ADT Fiat.ADTNotation Here.PipesFiat.
 
-Definition Stream (A : Type) := nat -> Comp A.
+Program Definition Spec := Def ADT {
+  rep := Producer nat unit,
 
-Definition nth_smallest `{StrictOrder A R} (n : nat) (s : Comp A) : Comp A :=
-  { i | exists xs, (In _ s i <-> List.In i xs)
-          /\ Sorted.Sorted R xs /\ i = List.nth n xs i }.
+  Def Constructor0 "empty" : rep :=
+    ret (empty _ _),,
 
-Definition map {A B} (f : A -> B -> Prop) (s : Stream A) : Stream B := fun n =>
-  { b : B | exists a, s n a /\ f a b }.
+  Def Method1 "add" (r : rep) (n : nat) : rep * nat :=
+    ret (forP r (fun x => yield (x + n)), n),
 
-Definition filter {A} (f : A -> Prop) (s : Stream A) : Stream A := fun n =>
-  i <- nth_smallest n { i | exists x, s i x /\ f x };
-  s i.
-
-Definition flatten {A} (s : Stream (Stream A)) : Stream A := fun n =>
-  `(i, j) <- nth_smallest n
-     { p | forall i j : nat, p = (i, j) -> exists s' x, s i s' /\ s' j x };
-  s' <- s i;
-  s' j.
-
-Definition bind {A B} (f : A -> Stream B -> Prop) (s : Stream A) : Stream B :=
-  flatten (map f s).
-
-Require Import Fiat.Computation.FixComp.
-Import LeastFixedPointFun.
-
-Definition foldr_spec `(f : B -> A -> A) (z : A) (s : Stream B) : Stream A :=
-  LeastFixedPoint (fDom:=[nat : Type]%list)
-    (fun rec pos =>
-       b <- s pos;
-       z' <- match pos with
-             | O => ret z
-             | S n => rec n
-             end;
-       ret (f b z')).
-
-(* A pipe connects two bi-directional streams and produces a result after a
-   number of steps. *)
-Record Pipe (A' A B' B R : Type) := mkPipe {
-  segment : (A' -> Stream A) -> (B -> Stream B') -> Comp R;
-  proper  :
-    Proper (pointwise_relation A' (pointwise_relation nat refine) ==>
-            pointwise_relation B  (pointwise_relation nat refine) ==>
-            refine) segment
-}.
-
-Arguments Pipe A' A B' B R.
-
-Definition refine_pipe `(x : Pipe A' A B' B R) (y : Pipe A' A B' B R) :=
-  forall inc out, refine (segment x inc out) (segment y inc out).
-
-Infix "=|" := refine_pipe (at level 100).
-
-Notation "()" := (unit : Type).
-
-Definition Void := False.
-
-Definition Producer := Pipe Void () ().
-
-Definition Producer' B R := forall {X' X}, Pipe X' X () B R.
-
-Program Definition yield {X' X A} (x : A) : Pipe X' X () A () :=
-  {| segment := fun _inc out => out x 0; proper := _ |}.
-Obligation 1.
-  intros ??????.
-  rewrite H0.
-  reflexivity.
-Qed.
-
-Program Definition forP `(p : Pipe x' x b' b a') `(f : b -> Pipe x' x c' c b') :
-  Pipe x' x c' c a' :=
-  {| segment :=
-       fun inc out =>
-         segment p inc
-                 (fun b i =>
-                    segment (f b) inc
-                            (fun c j =>
-                               n <- { n | exists s, nth_smallest n s (i, j) };
-                                 out c n))
-   ; proper := _ |}.
-Obligation 1.
-  intros ??????.
-  destruct p; simpl.
-  rewrite H.
-  f_equiv.
-  intros ??.
-  destruct (f a); simpl.
-  rewrite H.
-  setoid_rewrite H0.
-  reflexivity.
-Qed.
-
-Ltac compext :=
-  apply Extensionality_Ensembles;
-  split; intros; intros ??.
-
-Definition Spec := Def ADT {
-  rep := unit,
-
-  Def Constructor0 "empty" : rep := ret tt,,
-
-  Def Method0 "foo" (r : rep) : rep * nat :=
-    n <- { n : nat | n < 100 };
-    ret (r, n + 10)
+  Def Method0 "peel" (r : rep) : rep * option nat :=
+    p <- next r;
+    ret (match p with
+         | inl x => (empty _ _, None)
+         | inr (a, n) => (n, Some a)
+         end)
 }.
 
 Open Scope string_scope.
 
-Definition foo (r : Rep Spec) : Comp (Rep Spec * nat) :=
-  Eval simpl in let fooS := "foo" in callMeth Spec fooS r.
+Definition add (r : Rep Spec) (n : nat) : Comp (Rep Spec * nat) :=
+  Eval simpl in let addS := "add" in callMeth Spec addS r n.
 
 Inductive Term (c : Type) (a : Type) :=
   | Get   : (c -> Term c a) -> Term c a
@@ -121,20 +33,21 @@ Arguments Put {c a} _ _.
 Arguments Done {c a} _.
 Arguments Error {c a}.
 
-Inductive transformed {c a : Type} : Comp a -> Term c a -> Prop :=
+Inductive transformed {c a : Type} :
+  Comp (Producer c unit * a) -> Term c a -> Prop :=
   | TermGet   : forall (P : Comp c) k f,
       (* jww (2016-10-03): How do I relate [P] to a predicate on the value
          resulting from [Get]? *)
       (forall v, P v -> transformed (k v) (f v))
         -> transformed (z <- P; k z) (Get f)
   | TermPut   : forall ca s r, transformed ca r -> transformed ca (Put s r)
-  | TermDone  : forall b k (v : b), transformed (ret (k v)) (Done (k v))
+  | TermDone  : forall r b k (v : b), transformed (ret (r, k v)) (Done (k v))
   | TermError : forall ca, transformed ca Error.
 
 Hint Constructors transformed.
 
-Definition fooC (r : Rep Spec) : Comp (Rep Spec * nat) :=
-  Eval simpl in let fooS := "foo" in callMeth Spec fooS r.
+Definition addC (r : Rep Spec) (n : nat) : Comp (Rep Spec * nat) :=
+  Eval simpl in let addS := "add" in callMeth Spec addS r n.
 
 Ltac compileTerm :=
   repeat match goal with
@@ -142,18 +55,18 @@ Ltac compileTerm :=
   | [ |- transformed (ret _) _ ] => eapply TermDone
   end; intros.
 
-Lemma fooT : { f : Rep Spec -> Term nat (Rep Spec * nat)
-             & forall r, transformed (fooC r) (f r) }.
+Lemma addT : { f : nat -> Term nat nat
+             & forall r n, transformed (addC r n) (f n) }.
 Proof.
-  eexists.
-  unfold fooC; intros.
-  apply TermGet; intros.
-  (* A [Put] can be inserted anywhere, since it is orthogonal to the semantics
-     of the computation. *)
-  apply TermPut with (s:=20).
-  apply TermDone.
-Defined.
+  exists (fun n => Get (fun x => Put (x + n) (Done n))).
+  unfold addC; intros.
+  (* apply TermGet; intros. *)
+  (* (* A [Put] can be inserted anywhere, since it is orthogonal to the semantics *)
+  (*    of the computation. *) *)
+  (* apply TermPut with (s:=20). *)
+  (* apply TermDone. *)
+Admitted.
 
-Definition fooT' := Eval simpl in projT1 fooT.
-Print fooT'.
-(* fooT' = fun r : () => Get (fun v : nat => Put 20 (Done (r, v + 10))) *)
+Definition addT' := Eval simpl in projT1 addT.
+Print addT'.
+(* addT' = fun r : () => Get (fun v : nat => Put 20 (Done (r, v + 10))) *)
